Lean4Lean/Environment.lean
@@ -53,9 +53,9 @@ def addTheorem (env : Environment) (v : TheoremVal) (check := true) (fuel : Fuel
   if check then
     -- TODO(Leo): we must add support for handling tasks here
     M.run env (safety := .safe) (lctx := {}) (lparams := v.levelParams) (fuel := fuel) do
+      checkConstantVal env v.toConstantVal
       if !(← isProp v.type) then
         throw <| .thmTypeIsNotProp env v.name v.type
-      checkConstantVal env v.toConstantVal
       let valType ← TypeChecker.checkType v.value
       if !(← isDefEq valType v.type) then
         throw <| .declTypeMismatch env (.thmDecl v) valType
